ConNF/Counting/SpecSMul.lean
@@ -6,10 +6,193 @@ import ConNF.Counting.Spec
 
 open Quiver Set Sum WithBot
 
+open scoped symmDiff
+
 universe u
 
 namespace ConNF
 
-variable [Params.{u}] [Level] [FOAAssumptions] {β : Λ} [i : LeLevel β] {σ : Spec β} {S : Support β}
+variable [Params.{u}] [Level] [FOAAssumptions] {β : Λ} [LeLevel β]
+  {S T : Support β} {hS : S.Strong} {σ : Spec β} (hσS : σ.Specifies S hS) (ρ : Allowable β)
+
+theorem Support.Specifies.smul : σ.Specifies (ρ • S) (hS.smul ρ) := by
+  constructor
+  case max_eq_max => exact hσS.max_eq_max
+  case atom_spec =>
+    intro i hi A a ha
+    rw [hσS.atom_spec i hi A ((Allowable.toStructPerm ρ A)⁻¹ • a)]
+    swap
+    · rw [Enumeration.smul_f, smul_eq_iff_eq_inv_smul] at ha
+      rw [ha, Allowable.smul_address, map_inv, Tree.inv_apply, smul_inl]
+    simp only [Enumeration.smul_f, Enumeration.smul_max, SpecCondition.atom.injEq]
+    refine ⟨trivial, ?_, ?_⟩
+    · ext j
+      constructor
+      · rintro ⟨hj, hjS⟩
+        refine ⟨hj, ?_⟩
+        rw [hjS, Allowable.smul_address, smul_inl, smul_inv_smul]
+      · rintro ⟨hj, hjS⟩
+        refine ⟨hj, ?_⟩
+        rw [smul_eq_iff_eq_inv_smul] at hjS
+        rw [hjS, Allowable.smul_address, smul_inl, map_inv, Tree.inv_apply]
+    · ext j
+      constructor
+      · rintro ⟨hj₁, N, hj₂, hj₃⟩
+        refine ⟨hj₁, Allowable.toStructPerm ρ A • N, ?_, ?_⟩
+        · rw [hj₂, Allowable.smul_address, smul_inr]
+        · rw [← SetLike.mem_coe, NearLitterPerm.smul_nearLitter_coe,
+            mem_smul_set_iff_inv_smul_mem]
+          exact hj₃
+      · rintro ⟨hj₁, N, hj₂, hj₃⟩
+        refine ⟨hj₁, (Allowable.toStructPerm ρ A)⁻¹ • N, ?_, ?_⟩
+        · rw [smul_eq_iff_eq_inv_smul] at hj₂
+          rw [hj₂, Allowable.smul_address, smul_inr, map_inv, Tree.inv_apply]
+        · rw [← SetLike.mem_coe, NearLitterPerm.smul_nearLitter_coe,
+            mem_smul_set_iff_inv_smul_mem, inv_inv, smul_inv_smul, SetLike.mem_coe]
+          exact hj₃
+  case flexible_spec =>
+    intro i hi A N hN h
+    rw [hσS.flexible_spec i hi A ((Allowable.toStructPerm ρ A)⁻¹ • N)]
+    swap
+    · have := hN.smul ρ⁻¹
+      simp only [map_inv, Tree.inv_apply] at this
+      exact this
+    swap
+    · rw [Enumeration.smul_f, smul_eq_iff_eq_inv_smul] at h
+      rw [h, Allowable.smul_address, map_inv, Tree.inv_apply, smul_inr]
+    simp only [Enumeration.smul_f, Enumeration.smul_max, SpecCondition.flexible.injEq]
+    refine ⟨trivial, ?_, ?_⟩
+    · ext j
+      constructor
+      · rintro ⟨hj₁, N', hj₂, hj₃⟩
+        refine ⟨hj₁, Allowable.toStructPerm ρ A • N', ?_, ?_⟩
+        · rw [hj₂, Allowable.smul_address, smul_inr]
+        · rw [NearLitterPerm.smul_nearLitter_fst, hj₃,
+            NearLitterPerm.smul_nearLitter_fst, smul_inv_smul]
+      · rintro ⟨hj₁, N', hj₂, hj₃⟩
+        refine ⟨hj₁, (Allowable.toStructPerm ρ A)⁻¹ • N', ?_, ?_⟩
+        · rw [smul_eq_iff_eq_inv_smul] at hj₂
+          rw [hj₂, Allowable.smul_address, smul_inr, map_inv, Tree.inv_apply]
+        · simp only [NearLitterPerm.smul_nearLitter_fst, smul_left_cancel_iff]
+          exact hj₃
+    · ext j k
+      constructor
+      · rintro ⟨hj, hk, a, N', h₁, h₂, h₃, h₄⟩
+        refine ⟨hj, hk, Allowable.toStructPerm ρ A • a, Allowable.toStructPerm ρ A • N',
+            ?_, ?_, ?_, ?_⟩
+        · rw [NearLitterPerm.smul_nearLitter_fst, h₁,
+            NearLitterPerm.smul_nearLitter_fst, smul_inv_smul]
+        · rw [← mem_inv_smul_set_iff, smul_set_symmDiff,
+            ← NearLitterPerm.smul_nearLitter_coe, ← NearLitterPerm.smul_nearLitter_coe,
+            inv_smul_smul]
+          exact h₂
+        · rw [h₃, Allowable.smul_address, smul_inr]
+        · rw [h₄, Allowable.smul_address, smul_inl]
+      · rintro ⟨hj, hk, a, N', h₁, h₂, h₃, h₄⟩
+        refine ⟨hj, hk, (Allowable.toStructPerm ρ A)⁻¹ • a, (Allowable.toStructPerm ρ A)⁻¹ • N',
+            ?_, ?_, ?_, ?_⟩
+        · rw [NearLitterPerm.smul_nearLitter_fst, h₁,
+            NearLitterPerm.smul_nearLitter_fst]
+        · rw [← mem_inv_smul_set_iff, smul_set_symmDiff,
+            ← NearLitterPerm.smul_nearLitter_coe, ← NearLitterPerm.smul_nearLitter_coe,
+            inv_smul_smul, inv_inv, smul_inv_smul]
+          exact h₂
+        · rw [smul_eq_iff_eq_inv_smul] at h₃
+          rw [h₃, Allowable.smul_address, map_inv, Tree.inv_apply, smul_inr]
+        · rw [smul_eq_iff_eq_inv_smul] at h₄
+          rw [h₄, Allowable.smul_address, map_inv, Tree.inv_apply, smul_inl]
+  case inflexibleCoe_spec =>
+    rintro i hi A N ⟨P, t, ht⟩ hSi
+    rw [hσS.inflexibleCoe_spec i hi A ((Allowable.toStructPerm ρ A)⁻¹ • N)
+      ⟨P, (Allowable.comp (P.B.cons P.hδ) ρ)⁻¹ • t, ?_⟩]
+    swap
+    · rw [Enumeration.smul_f, smul_eq_iff_eq_inv_smul] at hSi
+      rw [hSi, Allowable.smul_address, map_inv, Tree.inv_apply, smul_inr]
+    swap
+    · have := (InflexibleCoe.smul ⟨P, t, ht⟩ ρ⁻¹).hL
+      simp only [map_inv, Tree.inv_apply, inflexibleCoe_smul_path, inflexibleCoe_smul_t] at this
+      exact this
+    rw [SpecCondition.inflexibleCoe.injEq]
+    refine ⟨rfl, HEq.rfl, heq_of_eq ?_, ?_⟩
+    · simp only [NearLitterPerm.smul_nearLitter_fst, inflexibleCoe_smul_path, inflexibleCoe_smul_t,
+        Tree.inv_apply, ne_eq, eq_mp_eq_cast, CodingFunction.code_eq_code_iff]
+      refine ⟨Allowable.comp (P.B.cons P.hδ) ρ, ?_, (smul_inv_smul _ _).symm⟩
+      simp only [before_smul, comp_smul, NearLitterPerm.smul_nearLitter_fst,
+        inflexibleCoe_smul_path, inflexibleCoe_smul_t, Tree.inv_apply, ne_eq, eq_mp_eq_cast]
+    · ext j k
+      constructor
+      · rintro ⟨hj, hk, a, N', h₁, h₂, h₃, h₄⟩
+        refine ⟨hj, hk, Allowable.toStructPerm ρ A • a, Allowable.toStructPerm ρ A • N',
+            ?_, ?_, ?_, ?_⟩
+        · rw [NearLitterPerm.smul_nearLitter_fst, h₁,
+            NearLitterPerm.smul_nearLitter_fst, smul_inv_smul]
+        · rw [← mem_inv_smul_set_iff, smul_set_symmDiff,
+            ← NearLitterPerm.smul_nearLitter_coe, ← NearLitterPerm.smul_nearLitter_coe,
+            inv_smul_smul]
+          exact h₂
+        · rw [Enumeration.smul_f, h₃, Allowable.smul_address, smul_inr]
+        · rw [Enumeration.smul_f, h₄, Allowable.smul_address, smul_inl]
+      · rintro ⟨hj, hk, a, N', h₁, h₂, h₃, h₄⟩
+        refine ⟨hj, hk, (Allowable.toStructPerm ρ A)⁻¹ • a, (Allowable.toStructPerm ρ A)⁻¹ • N',
+            ?_, ?_, ?_, ?_⟩
+        · rw [NearLitterPerm.smul_nearLitter_fst, h₁,
+            NearLitterPerm.smul_nearLitter_fst]
+        · rw [← mem_inv_smul_set_iff, smul_set_symmDiff,
+            ← NearLitterPerm.smul_nearLitter_coe, ← NearLitterPerm.smul_nearLitter_coe,
+            inv_smul_smul, inv_inv, smul_inv_smul]
+          exact h₂
+        · rw [Enumeration.smul_f, smul_eq_iff_eq_inv_smul] at h₃
+          rw [h₃, Allowable.smul_address, map_inv, Tree.inv_apply, smul_inr]
+        · rw [Enumeration.smul_f, smul_eq_iff_eq_inv_smul] at h₄
+          rw [h₄, Allowable.smul_address, map_inv, Tree.inv_apply, smul_inl]
+  case inflexibleBot_spec =>
+    rintro i hi A N ⟨P, a, ha⟩ hSi
+    rw [hσS.inflexibleBot_spec i hi A ((Allowable.toStructPerm ρ A)⁻¹ • N)
+      ⟨P, (Allowable.toStructPerm ρ (P.B.cons (bot_lt_coe _)))⁻¹ • a, ?_⟩]
+    swap
+    · rw [Enumeration.smul_f, smul_eq_iff_eq_inv_smul] at hSi
+      rw [hSi, Allowable.smul_address, map_inv, Tree.inv_apply, smul_inr]
+    swap
+    · have := (InflexibleBot.smul ⟨P, a, ha⟩ ρ⁻¹).hL
+      simp only [map_inv, Tree.inv_apply] at this
+      rw [NearLitterPerm.smul_nearLitter_fst, this, InflexibleBot.smul]
+      simp_rw [Allowable.comp_bot, map_inv, Tree.inv_apply]
+    rw [SpecCondition.inflexibleBot.injEq]
+    refine ⟨rfl, HEq.rfl, ?_, ?_⟩
+    · ext j
+      constructor
+      · rintro ⟨hj, hjS⟩
+        refine ⟨hj, ?_⟩
+        rw [Enumeration.smul_f, hjS, Allowable.smul_address, smul_inl, smul_inv_smul]
+      · rintro ⟨hj, hjS⟩
+        refine ⟨hj, ?_⟩
+        rw [Enumeration.smul_f, smul_eq_iff_eq_inv_smul] at hjS
+        simp_rw [hjS, Allowable.smul_address, smul_inl, map_inv, Tree.inv_apply]
+    · ext j k
+      constructor
+      · rintro ⟨hj, hk, a, N', h₁, h₂, h₃, h₄⟩
+        refine ⟨hj, hk, Allowable.toStructPerm ρ A • a, Allowable.toStructPerm ρ A • N',
+            ?_, ?_, ?_, ?_⟩
+        · rw [NearLitterPerm.smul_nearLitter_fst, h₁,
+            NearLitterPerm.smul_nearLitter_fst, smul_inv_smul]
+        · rw [← mem_inv_smul_set_iff, smul_set_symmDiff,
+            ← NearLitterPerm.smul_nearLitter_coe, ← NearLitterPerm.smul_nearLitter_coe,
+            inv_smul_smul]
+          exact h₂
+        · rw [Enumeration.smul_f, h₃, Allowable.smul_address, smul_inr]
+        · rw [Enumeration.smul_f, h₄, Allowable.smul_address, smul_inl]
+      · rintro ⟨hj, hk, a, N', h₁, h₂, h₃, h₄⟩
+        refine ⟨hj, hk, (Allowable.toStructPerm ρ A)⁻¹ • a, (Allowable.toStructPerm ρ A)⁻¹ • N',
+            ?_, ?_, ?_, ?_⟩
+        · rw [NearLitterPerm.smul_nearLitter_fst, h₁,
+            NearLitterPerm.smul_nearLitter_fst]
+        · rw [← mem_inv_smul_set_iff, smul_set_symmDiff,
+            ← NearLitterPerm.smul_nearLitter_coe, ← NearLitterPerm.smul_nearLitter_coe,
+            inv_smul_smul, inv_inv, smul_inv_smul]
+          exact h₂
+        · rw [Enumeration.smul_f, smul_eq_iff_eq_inv_smul] at h₃
+          rw [h₃, Allowable.smul_address, map_inv, Tree.inv_apply, smul_inr]
+        · rw [Enumeration.smul_f, smul_eq_iff_eq_inv_smul] at h₄
+          rw [h₄, Allowable.smul_address, map_inv, Tree.inv_apply, smul_inl]
 
 end ConNF
